设等比数列的前n项和为S(n), 等比数列的第一项为a1，比值为q。

（1）
$$
S(n) = a1 + a1 * q + a1 * q ^ 2 + .... + a1 * q ^ {(n - 1)};
$$

（2）
$$
S(n+1) = a1 + a1 * q + a1 * q ^ 2 + .... + a1 * q ^ {(n - 1)} + a1 * q ^ n;
$$

由（2）式减（1）式得
（3）
$$
S(n+1) - s(n) = a1 * q ^ n;
$$


由S(n) * q 得
（4）
$$
S(n) * q = a1 * q + a1 * q ^ 2 + ... + a1 * q ^ n;
$$

由（2）- （4）得
（5）
$$
S(n+1) - S(n) * q = a1;
$$

由（3） - （5） 得
$$
[S(n+1) - S(n)] - [S(n+1) - S(n) * q] = a1 * q ^ n - a1;
$$
化简得：
$$
S(n) * q - S(n) = a1 * (q ^ n - 1);
$$
即：
$$
S(n) = a1 * (q ^ n - 1) / (q - 1);
$$

